Define WP and several lemmas

clang/logic.v
@@ -1,4 +1,124 @@
 Require Import lang.
+From iris.base_logic Require Import gen_heap.
+From iris.algebra Require Import gmap agree auth.
+From iris.base_logic.lib Require Import wsat fancy_updates.
+From iris.proofmode Require Import tactics.
+Set Default Proof Using "Type".
+Import uPred.
+
+Class clangG Σ := ClangG {
+  clangG_invG :> invG.invG Σ;
+  clangG_memG :> gen_heapG block (list byteval) Σ
+}.
+
+Section definitions.
+  Context `{clangG Σ}.
+  
+  Definition wp_pre
+           (wp: coPset -c> code -c> (val -c> iProp Σ) -c> iProp Σ) :
+    coPset -c> code -c> (val -c> iProp Σ) -c> iProp Σ :=
+    (λ E c Φ,
+     (* value case *)
+     (∃ v, ⌜to_val c = Some v⌝ ∧ |={E}=> Φ v) ∨
+     (* step case *)
+     (⌜to_val c = None⌝ ∧
+      (∀ (σ: mem),
+         gen_heap_ctx σ ={E,∅}=∗
+           ⌜reducible c⌝ ∗
+           ▷ (∀ c' σ', ⌜head_step c σ c' σ'⌝ ={∅,E}=∗
+             gen_heap_ctx σ' ∗ wp E c' Φ))))%I.
+
+  Local Instance wp_pre_contractive : Contractive wp_pre.
+  Proof.
+    rewrite /wp_pre=> n wp wp' Hwp E e1 Φ.
+    repeat (f_contractive || f_equiv); apply Hwp.
+  Qed.
+
+  Definition wp_def :
+    coPset → code → (val → iProp Σ) → iProp Σ := fixpoint wp_pre.
+  Definition wp_aux : { x | x = @wp_def }. by eexists. Qed.
+  Definition wp := proj1_sig wp_aux.
+  Definition wp_eq : @wp = @wp_def := proj2_sig wp_aux.
+
+  Notation "'WP' c @ E {{ Φ } }" := (wp E c Φ)
+    (at level 20, c, Φ at level 200,
+     format "'WP'  c  @  E  {{  Φ  } }") : uPred_scope.
+  Notation "'WP' c {{ Φ } }" := (wp ⊤ c Φ)
+    (at level 20, c, Φ at level 200,
+     format "'WP'  c  {{  Φ  } }") : uPred_scope.
+
+  Notation "'WP' c @ E {{ v , Q } }" := (wp E c (λ v, Q))
+    (at level 20, c, Q at level 200,
+     format "'WP'  c  @  E  {{  v ,  Q  } }") : uPred_scope.
+  Notation "'WP' c {{ v , Q } }" := (wp ⊤ c (λ v, Q))
+    (at level 20, c, Q at level 200,
+     format "'WP'  c  {{  v ,  Q  } }") : uPred_scope.
+
+  Lemma wp_unfold E c Φ : WP c @ E {{ Φ }} ⊣⊢ wp_pre wp E c Φ.
+  Proof. rewrite wp_eq. apply (fixpoint_unfold wp_pre). Qed.
+
+  Lemma wp_value Φ v E: Φ v ⊢ WP (of_val v) @ E {{ Φ }}.
+  Proof.
+    iIntros "HΦ".
+    rewrite wp_unfold /wp_pre.
+    iLeft. iExists v. auto.
+  Qed.
+
+
+  Lemma wp_strong_mono E1 E2 c Φ Ψ :
+    E1 ⊆ E2 → (∀ v, Φ v ={E2}=∗ Ψ v) ∗ WP c @ E1 {{ Φ }} ⊢ WP c @ E2 {{ Ψ }}.
+  Proof.
+    iIntros (?) "[HΦ H]". iLöb as "IH" forall (c).
+    rewrite !wp_unfold /wp_pre.
+    iDestruct "H" as "[Hv|[% H]]"; [iLeft|iRight].
+    { iDestruct "Hv" as (v) "[% Hv]". iExists v; iSplit; first done.
+      iApply ("HΦ" with ">[-]"). by iApply (fupd_mask_mono E1 _). }
+    iSplit; [done|]; iIntros (σ1) "Hσ".
+    iMod (fupd_intro_mask' E2 E1) as "Hclose"; first done.
+    iMod ("H" $! σ1 with "Hσ") as "[$ H]".
+    iModIntro. iNext. iIntros (e2 σ2 Hstep).
+    iMod ("H" $! e2 σ2 with "[#]") as "($ & H)"; auto.
+    iMod "Hclose" as "_". by iApply ("IH" with "HΦ").
+  Qed.
+
+  Lemma fupd_wp E e Φ : (|={E}=> WP e @ E {{ Φ }}) ⊢ WP e @ E {{ Φ }}.
+  Proof.
+    rewrite wp_unfold /wp_pre. iIntros "H". destruct (to_val e) as [v|] eqn:?.
+    { iLeft. iExists v; iSplit; first done.
+        by iMod "H" as "[H|[% ?]]"; [iDestruct "H" as (v') "[% ?]"|]; simplify_eq. }
+      iRight; iSplit; [done|]; iIntros (σ1) "Hσ1".
+    iMod "H" as "[H|[% H]]"; last by iApply "H".
+    iDestruct "H" as (v') "[% ?]"; simplify_eq.
+  Qed.
+  Lemma wp_fupd E e Φ : WP e @ E {{ v, |={E}=> Φ v }} ⊢ WP e @ E {{ Φ }}.
+  Proof. iIntros "H". iApply (wp_strong_mono E); try iFrame; auto. Qed.
+
+  Lemma fill_step_inv K e1' σ1 e2 σ2 :
+    to_val (e1', knil) = None → head_step (e1', K) σ1 e2 σ2 →
+    ∃ e2', e2 = (e2', K) ∧ head_step (e1', knil) σ1 (e2', knil) σ2.
+  Admitted.
+
+  Lemma wp_contΦ E k s Φ:
+    WP (curs s, knil) @ E {{ v, WP (curs Sskip, k) @ E {{ Φ }} }}
+       ⊢ WP (curs s, k) @ E {{ Φ }}.
+  Admitted.
+
+  Lemma wp_conte E k e Φ:
+    WP (cure e, knil) @ E {{ v, WP (cure (Evalue v), k) @ E {{ Φ }} }}
+       ⊢ WP (cure e, k) @ E {{ Φ }}.
+  Admitted.
+
+  Lemma wp_bind e Ke ke ks E Φ:
+    WP (cure e, (Ke::ke, ks)) @ E {{ Φ }}
+       ⊢ WP (cure (fill_expr Ke e), (ke, ks)) @ E {{ Φ }}.
+  Admitted.
+
+  Lemma wp_bind_s e Ks ks E Φ:
+    WP (cure e, ([], Ks::ks)) @ E {{ Φ }}
+       ⊢ WP (curs (fill_stmts Ks e), ([], ks)) @ E {{ Φ }}.
+  Admitted.
+
+End definitions.
 
 Definition spec_state := nat. (* XXX: should be parameterized *)
 
